Request generator

theories/Encode.v
@@ -1,18 +1,22 @@
 From AsyncTest Require Export
      Classes
      Operator.
+From JSON Require Export
+     Operator.
 From HTTP Require Export
      Message
      Printer.
-Import
+Export
+  JNotations
   XNotations.
+
 Open Scope jexp_scope.
 
 Instance XEncode__Method : XEncode request_method :=
   jobj' (JSON__String ∘ method_to_string) "method".
 
-Definition encode__path   : XEncode path           := jobj "path".
-Definition encode__oquery : XEncode (option query) := jobj "query".
+Definition xencode__path   : XEncode path           := jobj "path".
+Definition xencode__oquery : XEncode (option query) := jobj "query".
 
 Instance XEncode__Scheme : XEncode http_scheme :=
   jobj' (JSON__String ∘ scheme_to_string) "scheme".
@@ -25,11 +29,11 @@ Instance XEncode__RequestTarget : XEncode request_target :=
   fun t =>
     match t with
     | RequestTarget__Origin p oq =>
-      jkv "origin" $ encode__path p + encode__oquery oq
+      jkv "origin" $ xencode__path p + xencode__oquery oq
     | RequestTarget__Absolute (URI s a p oq) =>
-      jkv "absolute" $ xencode s + xencode a + encode__path p + encode__oquery oq
+      jkv "absolute" $ xencode s + xencode a + xencode__path p + xencode__oquery oq
     | RequestTarget__Authority a => jkv "authority" $ xencode a
-    | RequestTarget__Asterisk => Jexp__Const JSON__Null
+    | RequestTarget__Asterisk => Jexp__Object []
     end.
 
 Instance XEncode__Version : XEncode http_version :=
@@ -39,3 +43,21 @@ Instance XEncode__Version : XEncode http_version :=
 Instance XEncode__RequestLine : XEncode request_line :=
   fun l => let 'RequestLine m t v := l in
         xencode m + jkv "target" (xencode t) + xencode v.
+
+Instance XEncode__Field : XEncode (field_line id) :=
+  fun f => let 'Field k v := f in
+         jobj k v.
+
+Close Scope jexp_scope.
+
+Open Scope json_scope.
+
+Instance Encode__Status : JEncode status_line :=
+  fun s => let 'Status v c op := s in
+         encode v + Encode.jobj "code" c + Encode.jobj "reason" op.
+
+Instance Encode__Response : JEncode (http_response id) :=
+  fun r => let 'Response l f ob := r in
+         encode l + Encode.jobj "fields" f + Encode.jobj "body" ob.
+
+Close Scope json_scope.
