theories/Codec.v
@@ -1,0 +1,14 @@
+From HTTP Require Export
+     Decode
+     Encode
+     Parser
+     Printer.
+
+Definition jreq_to_string : IR -> string :=
+  request_to_string ∘ request_of_json.
+
+Definition jres_to_string : IR -> string :=
+  response_to_string ∘ response_of_json.
+
+Definition parseJres : parser IR :=
+  encode <$> parseResponse.
