theories/Gen.v
@@ -1,0 +1,81 @@
+From SimpleIO Require Export
+     IO_Random
+     SimpleIO.
+From Coq Require Export
+     ExtrOcamlIntConv.
+From HTTP Require Export
+     Encode
+     Semantics.
+Export
+  JpathNotations.
+Open Scope json_scope.
+
+Definition io_choose_ {A} (default : IO A) (l : list A) : IO A :=
+  match l with
+  | [] => default
+  | a :: _ =>
+    i <- nat_of_int <$> ORandom.int (int_of_nat (length l));;
+    ret (nth i l a)
+  end.
+
+Definition io_choose' {A} (l : list A) : IO (nat * A) :=
+  match l with
+  | [] => failwith "Cannot choose from empty list"
+  | a :: _ =>
+    i <- nat_of_int <$> ORandom.int (int_of_nat (length l));;
+    ret (i, nth i l a)
+  end.
+
+Definition io_choose {A} : list A -> IO A :=
+  fmap snd ∘ io_choose'.
+
+Definition io_or {A} (x y : IO A) : IO A :=
+  b <- ORandom.bool tt;;
+  if b : bool then x else y.
+
+Definition gen_string' : IO string :=
+  io_choose ["Hello"; "World"].
+
+Fixpoint gen_many {A} (n : nat) (ma : IO A) : IO (list A) :=
+  match n with
+  | O => ret []
+  | S n' => liftA2 cons ma $ io_or (ret []) (gen_many n' ma)
+  end.
+
+Definition gen_string : IO string :=
+  String "~" ∘ String.concat "" <$> gen_many 3 gen_string'.
+
+Definition gen_path : server_state exp -> IO path :=
+  io_choose_ gen_string ∘ map fst.
+
+Definition gen_line (ss : server_state exp) : IO request_line :=
+  p <- gen_path ss;;
+  m <- io_choose [Method__GET; Method__PUT];;
+  ret (RequestLine m (RequestTarget__Origin p None) (Version 1 1)).
+
+Definition find_etag (tr : traceT) : IO jexp :=
+  io_choose_ (ret $ Jexp__Object []) $
+             findpath ("fields" -> "ETag" -> this) id tr.
+
+Definition gen_condition (tr : traceT) : IO jexp :=
+  condition <- io_choose ["If-Match"; "If-None-Match"];;
+  etag <- find_etag tr;;
+  ret (jkv condition etag).
+
+Definition host_localhost : jexp := xencode $ Field "Host" "localhost".
+Definition content_length (content : string) : jexp :=
+  xencode $ Field "Content-Length" $ to_string $ String.length content.
+
+Open Scope jexp_scope.
+
+Definition gen_request (ss : server_state exp) (tr : traceT) : IO jexp :=
+  l <- gen_line ss;;
+  f <- gen_condition tr;;
+  match request__method l with
+  | Method__PUT =>
+    content <- gen_string;;
+    ret (xencode l +
+         jkv "fields" (host_localhost + f + content_length content) +
+         jobj "body" content)
+  | _ => ret $ xencode l + jkv "fields" (host_localhost + f)
+  end.
